cfi/refinementAQ.v
@@ -4,7 +4,7 @@ Require Import lib.utils.
 Require Import lib.Coqlib.
 Require Import concrete.common.
 Require Import cfi.abstract.
-Require Import cfi.qa.
+Require Import cfi.symbolic.
 Require Import cfi.cfi_rules.
 Require Import symbolic.symbolic.
 Require Coq.Vectors.Vector.
@@ -12,121 +12,253 @@ Require Coq.Vectors.Vector.
 Set Implicit Arguments.
 
 Section Refinement.
+Import PartMaps.
 
-Context {mt : machine_types}
-        {ops : machine_ops mt}
+Context {t : machine_types}
+        {ops : machine_ops t}
         {opss : machine_ops_spec ops}
-        {ap : Abstract.abstract_params mt}
+        
+        {ap : Abstract.abstract_params t}
         {aps : Abstract.params_spec ap}
-        {sp : @SymbolicCFI.sym_cfi_params mt}.
 
-Variable valid_jmp : word mt -> word mt -> bool.
+        {smemory : Type}
+        {sm : partial_map smemory (word t) (atom (word t) (@cfi_tag t))}
+        {smems : axioms sm}
+
+        {sregisters : Type}
+        {sr : partial_map sregisters (reg t) (atom (word t) (@cfi_tag t))}
+        {sregs : axioms sr}.
+
+Variable valid_jmp : word t -> word t -> bool.
 
 (* Instantiate the symbolic machine with the CFI stuff*)
 Definition sym_params := SymbolicCFI.sym_cfi valid_jmp.
 
-Context {sps : @Symbolic.params_spec mt sym_params}.
-
-Variable atable : list (Abstract.syscall mt).
-Variable stable : list (@Symbolic.syscall mt sym_params).
+Variable atable : list (Abstract.syscall t).
+Variable stable : list (@Symbolic.syscall t sym_params).
 
 (*this should be replaced, when step_a is defined*)
-Variable step_a : @Symbolic.state mt sym_params -> @Symbolic.state mt sym_params -> Prop.
+Variable step_a : @Symbolic.state t sym_params -> @Symbolic.state t sym_params -> Prop.
 
+(*Probably not needed here*)
 Definition amachine := Abstract.abstract_cfi_machine atable valid_jmp.
 Definition smachine := SymbolicCFI.symbolic_cfi_machine stable step_a.
 
-Definition refine_dmemory (admem : Abstract.dmemory mt) (smem : @Symbolic.memory mt sym_params) :=
-  forall w (x : word mt),
-    Symbolic.get_mem smem w = Some x@DATA <->
-    Abstract.get_dmem admem w = Some x. 
+(*Refinement related definitions*)
+Definition refine_dmemory (admem : Abstract.dmemory t)
+                          (smem : smemory) :=
+  forall w (x : word t),
+    get smem w = Some x@DATA <->
+    get admem w = Some x. 
 
-Definition refine_imemory (aimem : Abstract.imemory mt) (smem : @Symbolic.memory mt sym_params) :=
+Definition refine_imemory (aimem : Abstract.imemory t)
+                          (smem : smemory) :=
   forall w x,
-    (forall id, Symbolic.get_mem smem w = Some x@(INSTR id) ->
-                Abstract.get_imem aimem w = Some x) /\
-    (exists id, Abstract.get_imem aimem w = Some x ->
-                Symbolic.get_mem smem w = Some x@(INSTR id)).
+    (exists id, get smem w = Some x@(INSTR id)) <->
+    get aimem w = Some x.
 
-Definition refine_registers (areg : Abstract.registers mt) (sreg : @Symbolic.registers mt sym_params) :=
-  forall n (x : word mt),
-    (forall ut, Symbolic.get_reg sreg n = Some x@ut ->
-                Abstract.get_reg areg n = Some x) /\
-    (exists ut, Abstract.get_reg areg n = Some x ->
-                Symbolic.get_reg sreg n = Some x@ut).
+Definition refine_registers (areg : Abstract.registers t)
+                            (sreg : sregisters) :=
+  forall n (x : word t),
+    (exists ut, get sreg n = Some x@ut) <->
+    get areg n = Some x.
 
-Definition refine_syscalls (atbl : list (Abstract.syscall mt)) (stbl : list (@Symbolic.syscall mt sym_params)) :=
+Definition refine_pc 
+           (apc : word t) 
+           (spc : atom (word t) (@Symbolic.tag t sym_params)) :=
+  apc = common.val spc.
+
+(*Some useless lemmas, just for sanity check -- probably to be removed*)
+Lemma xxx : forall tpc ti,
+    (tpc = DATA \/ tpc = INSTR None \/
+     (exists src dst, tpc = INSTR (Some src) /\
+                      ti = INSTR (Some dst) /\
+                      valid_jmp src dst = true)) <->
+    (forall src, tpc = INSTR (Some src) ->
+       exists dst, ti = INSTR (Some dst) /\ valid_jmp src dst = true).
+Proof.
+  split.
+  - intro H.
+    destruct H as [? | [? | [src [dst [TPC [TI VALID]]]]]]; try (intros; congruence).
+    intros src0 TPC'.
+    rewrite TPC in TPC'. inversion TPC'; subst.
+    eexists; eauto.
+  - intros H.
+    destruct tpc.
+    + right. destruct o.
+      * right.
+        assert (H' := H w).
+        destruct H' as [dst [? ?]]. reflexivity.
+        eexists; eexists; eauto.
+      * left; reflexivity.
+    + left; reflexivity.
+Qed.
+
+Lemma yyy : forall tpc ti,
+   match tpc with
+   | INSTR (Some src) =>
+     exists dst, ti = INSTR (Some dst) /\ valid_jmp src dst = true
+   | _ => True
+   end
+    <->
+    (forall src, tpc = INSTR (Some src) ->
+       exists dst, ti = INSTR (Some dst) /\ valid_jmp src dst = true).
+Proof.
+  intros tpc ti.
+  split.
+  - destruct tpc.
+    * destruct o.
+      + intros H src H'. inversion H'; subst. assumption.
+      + intros ? src CONTRA. inversion CONTRA.
+    * intros ? ? CONTRA; inversion CONTRA.
+  - intros H. 
+    destruct tpc.
+    * destruct o.
+      + apply H; reflexivity.
+      + auto.
+    * auto.
+Qed.
+
+Definition refine_state (ast : Abstract.state t)
+                        (sst : @Symbolic.state t sym_params) :=
+  let '(imem, dmem, aregs, apc, cont) := ast in
+  let '(Symbolic.State smem sregs spc@tpc _) := sst in
+  refine_imemory imem smem /\
+  refine_dmemory dmem smem /\
+  refine_registers aregs sregs /\
+  refine_pc apc (spc@tpc) /\ (* not requiring anything about tpc? *)
+  forall i ti,
+    get smem spc = Some i@ti ->
+    (cont = true <->
+    (forall src, tpc = INSTR (Some src) ->
+       exists dst, ti = INSTR (Some dst) /\ valid_jmp src dst = true)).
+
+Definition refine_syscall acall scall :=
+  forall ast sst ares sres,
+    refine_state ast sst ->
+    acall ast = Some ares ->
+    scall sst = Some sres ->
+    refine_state ares sres.
+
+Definition same_domain
+           (atbl : list (Abstract.syscall t))
+           (stbl : list (@Symbolic.syscall t sym_params)) : Prop :=
   forall addr,
-    (forall sc, Symbolic.get_syscall stbl addr = Some sc ->
-                exists sc', Abstract.get_syscall atbl addr = Some sc') /\
-    (forall sc, Abstract.get_syscall atbl addr = Some sc ->
-                exists sc', Symbolic.get_syscall stbl addr = Some sc').
+    (exists acall, Abstract.get_syscall atbl addr = Some acall) <->
+    (exists scall, Symbolic.get_syscall stbl addr = Some scall).
 
-Definition refine_normal_state (ast : Abstract.state mt) (sst : Symbolic.state mt) :=
-  let '(Symbolic.State mem regs pc@tpc _) := sst in
-  let '(imem, dmem, aregs, apc, b) := ast in
-  b = true /\
-  pc = apc /\
-  refine_imemory imem mem /\
-  refine_dmemory dmem mem /\
-  refine_registers aregs regs /\
-  refine_syscalls atable stable.
+Lemma same_domain_total :
+  forall atbl stbl,
+    same_domain atbl stbl ->
+    forall addr', Abstract.get_syscall atbl addr' = None <-> 
+                  Symbolic.get_syscall stbl addr' = None.
+Proof.
+  intros atbl stbl SAME addr'.
+  assert (ACALL: forall addr'', Abstract.get_syscall atbl addr'' = None \/
+                         exists ac, Abstract.get_syscall atbl addr'' = Some ac).
+  { intros addr'';
+    destruct (Abstract.get_syscall atbl addr'');
+    [right; eexists; eauto | left; reflexivity].
+  }
+  assert (SCALL: forall addr'', Symbolic.get_syscall stbl addr'' = None \/
+                         exists sc, Symbolic.get_syscall stbl addr'' = Some sc).
+  { intros addr''.
+    destruct (Symbolic.get_syscall stbl addr'');
+      [right; eexists; eauto | left; reflexivity].
+  }
+  split.
+  - intro ACALL'. 
+    destruct (SCALL addr') as [? | CONTRA]; 
+      [assumption | apply SAME in CONTRA; destruct CONTRA; congruence].
+  - intro SCALL'.
+    destruct (ACALL addr') as [? | CONTRA]; 
+      [assumption | apply SAME in CONTRA; destruct CONTRA; congruence].
+Qed.
 
-Definition refine_violation_state (ast : Abstract.state mt) (sst : Symbolic.state mt) :=
-  let '(imem, dmem, aregs, apc, b) := ast in
-  b = false /\
-  exists ast0 sst0, 
-    let '(_, _, _, apc0, b0) := ast0 in
-    b0 = true /\
-    Abstract.step atable valid_jmp ast0 ast /\
-    Symbolic.step stable sst0 sst /\
-    refine_normal_state ast0 sst0 /\
-    valid_jmp apc0 apc = false.
+(* Might need absence of duplicates in these maps? *)
+Definition refine_syscalls 
+           (atbl : list (Abstract.syscall t))
+           (stbl : list (@Symbolic.syscall t sym_params)) : Prop :=
+  same_domain atbl stbl /\
+  forall addr acall scall,
+    Abstract.get_syscall atbl addr = Some acall ->
+    Symbolic.get_syscall stbl addr = Some scall ->
+    refine_syscall (@Abstract.sem t ap acall)
+                   (@Symbolic.sem t sym_params scall).
 
-Definition refine_state ast sst := 
-  refine_normal_state ast sst \/ refine_violation_state ast sst.
+Hypothesis refine_syscalls_correct : refine_syscalls atable stable.
+
+Hypothesis syscalls_backwards_simulation :
+  forall ast sst addr sc sst',
+    refine_syscalls atable stable ->
+    Symbolic.get_syscall stable addr = Some sc ->
+    refine_state ast sst ->
+    Symbolic.sem sc sst = Some sst' ->
+    exists ac ast',
+      Abstract.get_syscall atable addr = Some ac /\
+      Abstract.sem ac ast = Some ast' /\
+      refine_state ast' sst'.
+
+Hypothesis syscall_sem :
+  forall ac ast ast',
+    Abstract.sem ac ast = Some ast' ->
+       let '(imem,dmem,aregs,pc,b) := ast in
+       let '(imem',dmem',aregs',pc',b') := ast' in
+         imem = imem' /\ pc' = (pc + Z_to_word 1)%w /\ b' = b.
+
+(*Various hypothesis on how instructions are tagged*)
 
 Hypothesis id_hypothesis :
-  forall pc (w : word mt) (mem : @Symbolic.memory mt sym_params) id, 
-    Symbolic.get_mem mem pc = Some w@(INSTR (Some id)) ->
+  forall pc (w : word t) (mem : @Symbolic.memory t sym_params) id, 
+    get mem pc = Some w@(INSTR (Some id)) ->
     id = pc.
 
 Hypothesis jump_tagged :
-  forall pc w smem aimem r,
-    Abstract.get_imem aimem pc = Some w ->
-    decode_instr w = Some (Jump _ r) ->
-    refine_imemory aimem smem ->
-    Symbolic.get_mem smem pc = Some w@(INSTR (Some pc)).
+  forall pc i (mem : @Symbolic.memory t sym_params) r itg,
+    get mem pc = Some i@(INSTR itg) ->
+    decode_instr i = Some (Jump _ r) ->
+    itg = Some pc.
 
 Hypothesis jal_tagged :
-  forall pc w smem aimem r,
-    Abstract.get_imem aimem pc = Some w ->
-    decode_instr w = Some (Jal _ r) ->
-    refine_imemory aimem smem ->
-    Symbolic.get_mem smem pc = Some w@(INSTR (Some pc)).
+  forall pc i (mem : @Symbolic.memory t sym_params) r itg,
+    get mem pc = Some i@(INSTR itg) ->
+    decode_instr i = Some (Jal _ r) ->
+    itg = Some pc.
 
-Hypothesis jump_targets_tagged :
-  forall pc i smem regs r w (ti ti' : @Symbolic.tag mt sym_params),
-    Symbolic.get_mem smem pc = Some i@ti ->
+Hypothesis jump_target_tagged :
+  forall pc w (mem : @Symbolic.memory t sym_params) i i0 id r reg 
+         (tr ti : @Symbolic.tag t sym_params),
+    get mem pc = Some i@(INSTR (Some id)) ->
     decode_instr i = Some (Jump _ r) ->
-    Symbolic.get_reg regs r = Some w@ti' ->
-    ti' = INSTR (Some w).
+    get reg r = Some w@tr ->
+    get mem w = Some i0@ti ->
+    ti = INSTR (Some w).
 
+Hypothesis jal_target_tagged :
+  forall pc w (mem : @Symbolic.memory t sym_params) i i0 id r reg 
+         (tr ti : @Symbolic.tag t sym_params),
+    get mem pc = Some i@(INSTR (Some id)) ->
+    decode_instr i = Some (Jal _ r) ->
+    get reg r = Some w@tr ->
+    get mem w = Some i0@ti ->
+    Symbolic.get_syscall stable w = None ->
+    ti = INSTR (Some w).
 
 Import Vector.VectorNotations.
 
-Lemma refine_registers_upd sreg sreg' areg r v t v' t' :
+Lemma refine_registers_upd sreg sreg' areg r v tg v' tg' :
   refine_registers areg sreg ->
-  Symbolic.get_reg sreg r = Some v@t ->
-  Symbolic.upd_reg sreg r v'@t' = Some sreg' ->
+  get sreg r = Some v@tg ->
+  upd sreg r v'@tg' = Some sreg' ->
   exists areg',
-    Abstract.upd_reg areg r v' = Some areg' /\
+    upd areg r v' = Some areg' /\
     refine_registers areg' sreg'.
 Proof.
-  intros REFR GET UPD. unfold refine_registers in REFR.
-  destruct (REFR r v) as [REGSA REGAS].
-  apply REGSA in GET.
-  assert (NEW := PartMaps.upd_defined v' GET).
+  intros REFR GET UPD. 
+  assert (EGET: exists ut, get sreg r = Some v@ut) 
+    by (eexists; eassumption).
+  apply REFR in EGET.
+  assert (NEW := PartMaps.upd_defined v' EGET).
   destruct NEW as [areg' UPD'].
   eexists; split; eauto.
   unfold refine_registers. intros r' v''.
@@ -135,8 +267,8 @@ Proof.
     rewrite (PartMaps.get_upd_eq UPD').
     rewrite (PartMaps.get_upd_eq UPD). 
     split. 
-    - intros ut H. inversion H; reflexivity.
-    - exists t'. intro H1; inversion H1; auto.
+    - intro H. destruct H as [ut H]. inversion H; reflexivity.
+    - intro H. exists tg'; inversion H; reflexivity.
   * rewrite (PartMaps.get_upd_neq NEQ UPD).
     rewrite (PartMaps.get_upd_neq NEQ UPD').
     auto.
@@ -144,14 +276,14 @@ Qed.
 
 Lemma refine_memory_upd smem smem' amemd addr v v' :
   refine_dmemory amemd smem ->
-  Symbolic.get_mem smem addr = Some v@DATA ->
-  Symbolic.upd_mem smem addr v'@DATA = Some smem' ->
+  get smem addr = Some v@DATA ->
+  upd smem addr v'@DATA = Some smem' ->
   exists amemd',
-    Abstract.upd_dmem amemd addr v' = Some amemd' /\
+    upd amemd addr v' = Some amemd' /\
     refine_dmemory amemd' smem'.
 Proof.
-  intros MEM GET UPD. unfold refine_dmemory in MEM.
-  assert (GET': Abstract.get_dmem amemd addr = Some v) 
+  intros MEM GET UPD. 
+  assert (GET': get amemd addr = Some v) 
     by (apply MEM in GET; auto).
   destruct (PartMaps.upd_defined v' GET') as [amem' UPD'].
   do 2 eexists; eauto.
@@ -165,12 +297,12 @@ Proof.
     now apply MEM.
 Qed.
 
-Lemma data_memory_upd (smem : @Symbolic.memory mt sym_params) smem' addr v v' :
-  Symbolic.get_mem smem addr = Some v@DATA -> 
-  Symbolic.upd_mem smem addr v'@DATA = Some smem' ->
+Lemma data_memory_upd (smem : @Symbolic.memory t sym_params) smem' addr v v' :
+  get smem addr = Some v@DATA -> 
+  upd smem addr v'@DATA = Some smem' ->
   (forall addr' i id, 
-     Symbolic.get_mem smem addr' = Some i@(INSTR id) ->
-     Symbolic.get_mem smem' addr' = Some i@(INSTR id)).
+     get smem addr' = Some i@(INSTR id) ->
+     get smem' addr' = Some i@(INSTR id)).
 Proof.
   intros GET UPD addr' i id GET'.
   destruct (addr' == addr) as [EQ | NEQ]; [simpl in EQ | simpl in NEQ]; subst.
@@ -179,33 +311,29 @@ Proof.
     assumption.
 Qed.
 
-Lemma imem_upd_preservation amemi (smem : @Symbolic.memory mt sym_params) (smem' : @Symbolic.memory mt sym_params) addr v v':
+Lemma imem_upd_preservation amemi (smem : @Symbolic.memory t sym_params) 
+      (smem' : @Symbolic.memory t sym_params) addr v v' :
   refine_imemory amemi smem ->
-  Symbolic.get_mem smem addr = Some v@DATA ->
-  Symbolic.upd_mem smem addr v'@DATA = Some smem' ->
+  get smem addr = Some v@DATA ->
+  upd smem addr v'@DATA = Some smem' ->
   refine_imemory amemi smem'.
 Proof.
   intros MEM GET UPD w x.
-  destruct (MEM w x) as [MEMSA MEMAS].
   split.
-  - intros id GET'.
+  - intros (id & GET').
     destruct (addr == w) as [EQ | NEQ]; [simpl in EQ | simpl in NEQ]; subst.
     * assert (CONTRA := PartMaps.get_upd_eq UPD).
-      rewrite CONTRA in GET'. discriminate.
+      simpl in CONTRA. rewrite CONTRA in GET'. discriminate.
     * eapply PartMaps.get_upd_neq in UPD; eauto.
-      Focus 2. apply sps.
-      rewrite UPD in GET'.
-      eapply MEMSA; eauto.
-  - destruct MEMAS as [id' H].
-    exists id'.
-    intro GET'. apply H in GET'.
+      simpl in UPD. rewrite UPD in GET'.
+      eapply MEM; eauto.
+  - intro GET'.
+    apply MEM in GET'.
     destruct (addr == w) as [EQ | NEQ]; [simpl in EQ | simpl in NEQ]; subst.
-    * rewrite GET in GET'. discriminate.
-    * eapply PartMaps.get_upd_neq in UPD; eauto. Focus 2. apply sps.
+    * simpl in GET. rewrite GET in GET'. destruct GET'; congruence.
+    * eapply PartMaps.get_upd_neq in UPD; eauto; simpl in UPD;
       rewrite UPD; assumption.
 Qed.
-
-Hint Resolve imem_upd_preservation.
 
 Ltac match_inv :=
   repeat match goal with
@@ -226,390 +354,6 @@ Ltac match_inv :=
   | H : True |- _ => clear H
   end.
 
-Theorem backwards_simulation_normal ast sst sst' :
-  refine_normal_state ast sst ->
-  Symbolic.step stable sst sst' ->
-  exists ast',
-    Abstract.step atable valid_jmp ast ast' /\
-    refine_state ast' sst'.
-Proof.
-  intros REF SSTEP.
-  destruct ast as [[[[imem dmem] aregs] apc] b].
-  destruct b; [idtac | inversion SSTEP; subst; destruct REF; discriminate].
-  inversion SSTEP; subst;
-  destruct REF as [? [? [? [? ?]]]]; subst apc;
-  (*unfoldings and case analysis on tags*)
-  repeat (
-      match goal with
-        | [H: Symbolic.next_state_pc _ _ _ = _ |- _] => unfold Symbolic.next_state_pc in H
-        | [H: Symbolic.next_state_reg _ _ _ _ = _ |- _] => unfold Symbolic.next_state_reg in H
-        | [H: Symbolic.next_state_reg_and_pc _ _ _ _ _ = _ |- _] => 
-          unfold Symbolic.next_state_reg_and_pc in H
-        | [H: Symbolic.next_state _ _ _ = Some _ |- _] =>
-          unfold Symbolic.next_state in H; simpl in H; match_inv
-      end);
-  (* switch memory updates to abstract*)
-  repeat (
-      match goal with
-        | [H: SymbolicCFI.upd_mem ?Mem ?Addr ?V@_ = Some _, H1 : refine_dmemory _ ?Mem, 
-          H2: Symbolic.get_mem ?Mem ?Addr = Some _ |- _] => 
-          simpl in H; destruct (refine_memory_upd Addr V H1 H2 H) as [dmem' [? ?]]
-  end);
-
-  (*switch memory and register reads to abstract*)
-  repeat  match goal with
-    | [H1: refine_imemory _ _, H2: Symbolic.get_mem _ _ = Some _@(INSTR _) |- _] =>
-      apply H1 in H2
-    | [H1: refine_dmemory _ _, H2: Symbolic.get_mem _ _ = Some _@DATA |- _] => 
-      apply H1 in H2
-    | [H1: refine_registers _ _, H2: Symbolic.get_reg _ _ = Some _ |- _] => 
-      apply H1 in H2
-  end;
-        
-  repeat match goal with
-    | [H: refine_registers ?Aregs ?Regs, H1: Abstract.get_reg _ ?R = Some ?Old |- _] => 
-      unfold refine_registers in H; destruct (H R Old) as [RSA RAS]; destruct RAS as [x RAS'];
-      apply RAS' in H1; fold (refine_registers Aregs Regs) in H
-    | [H: refine_registers _ _, H1: Symbolic.get_reg ?Reg ?R = Some _,
-                                    H2: SymbolicCFI.upd_reg _ ?R ?V'@?T' = Some _ |- _] =>
-      destruct (refine_registers_upd R V' T' H H1 H2) as [aregs' [? ?]]
-    
-  end; auto;
-
-  (*handle abstract steps*)
-  repeat (match goal with 
-    | [|- exists _,  _ /\ _] => eexists; split
-    | [|- Abstract.step _ _ _ _] => econstructor(eassumption)
-    | [H: decode_instr _ = Some (Load _ _ _) |- Abstract.step _ _ _ _] => 
-      eapply Abstract.step_load; eauto
-    | [H: Symbolic.get_mem _ ?Addr = _, H1: refine_imemory _ _, H2: refine_dmemory _ _ 
-       |- Abstract.get_imem _ ?Addr =  _ \/ Abstract.get_dmem _ ?Addr = _] => (*for load*)
-      destruct t2; [left; apply H1 in H; eassumption | right; apply H2 in H; eassumption]
-    | [H: decode_instr _ = Some (Store _ _ _) |- Abstract.step _ _ _ _] => 
-      eapply Abstract.step_store; eauto
-    | [H: decode_instr _ = Some (Jump _ _ ) |- Abstract.step _ _ _ _] => 
-      eapply Abstract.step_jump; eauto
-    | [H: decode_instr _ = Some (Bnz _ _ _) |- Abstract.step _ _ _ _] =>
-      eapply Abstract.step_bnz; eauto
-    | [H: decode_instr _ = Some (Jal _ _ ) |- Abstract.step _ _ _ _] =>
-      eapply Abstract.step_jal; eauto
-         end);
-
-  (*handle final state refinement*)
-  repeat (match goal with
-    | [H: decode_instr _ = Some (Jump _ _) |- refine_state (_,_,_,_, valid_jmp ?Pc ?W) _] =>
-      remember (valid_jmp Pc W) as b; destruct b; [left; unfold refine_normal_state; repeat (split; auto) | idtac]
-    | [H: false = valid_jmp ?Pc ?W |- refine_state (_,_,_,_, false) _] =>
-      right; unfold refine_violation_state
-    | [|- _ /\ _] => split; [eauto | idtac]
-    | [|- exists _ _, _] => exists (imem,dmem,aregs,pc,true)
-    | [|- exists _, _] => eexists
-    | [H: decode_instr _ = Some (Jump _ _) |- Abstract.step _ _ _ (_,_,_,_,false)] =>
-      eapply Abstract.step_jump; eauto
-    | [|- refine_state (_,_,_,_,true) _] => left 
-    | [|- refine_normal_state _ _] => unfold refine_normal_state; simpl
-    | [H: refine_imemory ?Imem ?Mem |- refine_imemory ?Imem ?Mem] => assumption
-    | [H: refine_imemory ?Imem ?Mem |- refine_imemory ?Imem ?Mem'] => 
-        eapply imem_upd_preservation; eauto
-   end); 
-  repeat match goal with
-           | [H: refine_dmemory dmem ?Mem |- Symbolic.get_mem ?Mem _ = Some _] => eapply H; eauto
-         end; auto. 
-
-(*TODO: SYSTEM CALLS*)
-Admitted.           
-
-Lemma imem_refined_instructions mem imem pc i i' ut :
-  refine_imemory imem mem ->
-  Abstract.get_imem imem pc = Some i ->
-  Symbolic.get_mem mem pc = Some i'@ut ->
-  decode_instr i = decode_instr i'.
-Proof.
-  intros MEM GET GET'.
-  destruct (MEM pc i).
-  destruct H0. apply H0 in GET. rewrite GET in GET'. inversion GET'. subst. reflexivity.
-Qed.
-
-Lemma reg_refined_values reg areg r v v' ut :
-  refine_registers areg reg ->
-  Abstract.get_reg areg r = Some v ->
-  Symbolic.get_reg reg r = Some v'@ut ->
-  v = v'.
-Proof.
-  intros REG GET GET'.
-  destruct (REG r v). destruct H0. apply H0 in GET.
-  rewrite GET in GET'. inversion GET'. reflexivity.
-Qed.
-
-
-Theorem backwards_simulation_violation ast sst sst' :
-  refine_violation_state ast sst ->
-  Symbolic.step stable sst sst' ->
-  exists ast',
-    Abstract.step atable valid_jmp ast ast' /\
-    refine_state ast' sst'.
-Proof.
-   intros REF SSTEP.
-  destruct ast as [[[[imem dmem] aregs] apc] b].
-  destruct b; [inversion SSTEP; subst; destruct REF; discriminate | idtac].
-  destruct sst.
-  destruct REF as [? [ast0 [sst0 REF]]].
-  destruct ast0 as [[[[imem0 dmem0] aregs0] apc0] b0].
-  destruct REF as [B0 [ASTEP0 [SSTEP0 [REF0 INVALID]]]];
-  destruct sst0 as [mem0 regs0 [pc0 tpc0] ?]; 
-  destruct REF0 as [? [PC0EQ [REFI0 [REFD0 [REFR0 REFS0]]]]]; subst;
-  inversion ASTEP0;
-  inversion SSTEP0; inversion ST; subst; clear ST;
-  (*uninteresting cases*)
-    match goal with 
-        | [H: refine_imemory ?Imem ?Mem, H1: Abstract.get_imem ?Imem ?Pc = Some ?I,
-           H2: Symbolic.get_mem ?Mem ?Pc = Some ?I'@_ |- _] => 
-          destruct (imem_refined_instructions Pc H H1 H2); try congruence
-    end. Focus 3.
-  match goal with 
-      [H: decode_instr ?I = Some ?V, H': decode_instr ?I = Some ?V' |- _] => 
-      assert (EQINSTR: V = V') by (rewrite H in H'; inversion H'; auto); inversion EQINSTR;
-      subst; clear EQINSTR
-  end. 
-  
-
-  match goal with
-      | [H: Abstract.get_reg ?Aregs ?R = Some ?V, H': Symbolic.get_reg ?Sregs ?R' = Some ?V'@_,
-         H1: refine_registers ?Aregs ?Sregs |- _] =>
-        apply H1 in H'
-  end.
-  unfold refine_syscalls in REFS0. apply REFS0 in GETCALL0. destruct GETCALL0. rewrite GETCALL in H1.
-  
-  rewrite INST0 in INST. inversion INST. subst.
-  apply REFR0 in RW0. rewrite RW0 in RW. inversion RW. subst.
-  unfold refine_syscalls in REFS0.
-  destruct (REFS0 apc). 
-  apply H1 in GETCALL0. destruct GETCALL0. rewrite GETCALL in H3. inversion H3.
-  
-  unfold refine_registers in REFR0.
-  destruct ti; [idtac | simpl in ALLOWED; match_inv]. 
-   match goal with
-    | [H: Abstract.get_imem ?Imem ?Pc = Some ?I, H': Symbolic.get_mem ?Smem ?Pc = Some ?I'@(INSTR ?ID),
-       H1: refine_imemory ?Imem ?Smem |- _] => 
-      assert (I = I') by (apply H1 in H'; rewrite H' in H; inversion H; reflexivity); subst
-    | [H: Abstract.get_reg ?Aregs ?R = Some ?V, H': Symbolic.get_reg ?Sregs ?R' = Some ?V'@_,
-      H1: refine_registers ?Aregs ?Sregs |- _] =>
-      apply H1 in H'
-  end.
-   match goal with 
-         [H: decode_instr ?I = Some ?V, H': decode_instr ?I = Some ?V' |- _] => 
-         assert (EQINSTR: V = V') by (rewrite H in H'; inversion H'; auto); inversion EQINSTR;
-         subst; clear EQINSTR
-   end.
-
-
-
-
-  intros REF SSTEP.
-  destruct ast as [[[[imem dmem] aregs] apc] b].
-  destruct b; [inversion SSTEP; subst; destruct REF; discriminate | idtac];
-  inversion SSTEP; subst;
-  destruct REF as [? [ast0 [sst0 REF]]];
-  destruct ast0 as [[[[imem0 dmem0] aregs0] apc0] b0];
-  destruct REF as [B0 [ASTEP0 [SSTEP0 [REF0 INVALID]]]]; subst;
-  destruct sst0 as [mem0 regs0 [pc0 tpc0] ?]; 
-  destruct REF0 as [? [PC0EQ [REFI0 [REFD0 [REFR0 REFS0]]]]]; subst;
-  inversion ASTEP0;
-  inversion SSTEP0; inversion ST; subst;
-  (*uninteresting cases*)
-    match goal with 
-        | [H: refine_imemory ?Imem ?Mem, H1: Abstract.get_imem ?Imem ?Pc = Some ?I,
-           H2: Symbolic.get_mem ?Mem ?Pc = Some ?I'@_ |- _] => 
-          destruct (imem_refined_instructions Pc H H1 H2); try congruence
-    end;
-    (*unfoldings and case analysis on tags*)
-  repeat (
-      match goal with
-        | [H: Symbolic.next_state_pc _ _ _ = _ |- _] => unfold Symbolic.next_state_pc in H
-        | [H: Symbolic.next_state_reg _ _ _ _ = _ |- _] => unfold Symbolic.next_state_reg in H
-        | [H: Symbolic.next_state_reg_and_pc _ _ _ _ _ = _ |- _] => 
-          unfold Symbolic.next_state_reg_and_pc in H
-        | [H: Symbolic.next_state _ _ _ = Some _ |- _] =>
-          unfold Symbolic.next_state in H; simpl in H
-      end). Focus 4. rewrite CA
-
-  
-destruct ast0 as [[[[imem0 dmme0] aregs0] apc0] b0].
-  destruct REF as [B0 [ASTEP0 [SSTEP0 [REF0 INVALID]]]]; subst.
-  unfold Symbolic.next_state_pc in NEXT. unfold Symbolic.next_state in NEXT.
-  simpl in NEXT. 
-  destruct sst0 as [mem0 regs0 [pc0 tpc0] ?].
-  destruct REF0 as [? [PC0EQ [REFI0 [REFD0 REFR0]]]]; subst.
-  inversion ASTEP0; subst.
-
-  repeat (
-      match goal with
-        | [H: refine_violation_state _ _ => destruct H as [? [? [? ?]]]
-        | [H: 
-
- (*unfoldings and case analysis on tags*)
-  repeat (
-      match goal with
-        | [H: Symbolic.next_state_pc _ _ _ = _ |- _] => unfold Symbolic.next_state_pc in H
-        | [H: Symbolic.next_state_reg _ _ _ _ = _ |- _] => unfold Symbolic.next_state_reg in H
-        | [H: Symbolic.next_state_reg_and_pc _ _ _ _ _ = _ |- _] => 
-          unfold Symbolic.next_state_reg_and_pc in H
-        | [H: Symbolic.next_state _ _ _ = Some _ |- _] =>
-          unfold Symbolic.next_state in H; simpl in H; match_inv
-      end);
-
-
-
-  * (*case amachine took a jump*)
-     inversion SSTEP0; inversion ST; subst;
-    (*uninteresting cases*)
-    match goal with 
-        | [H: refine_imemory ?Imem ?Mem, H1: Abstract.get_imem ?Imem ?Pc = Some ?I,
-           H2: Symbolic.get_mem ?Mem ?Pc = Some ?I'@_ |- _] => 
-          destruct (imem_refined_instructions Pc H H1 H2); try congruence
-    end. 
-     (*case smachine took a jump too*)
-     unfold Symbolic.next_state_pc in NEXT0.
-     unfold Symbolic.next_state in NEXT0. simpl in NEXT0.
-     assert (GET := jump_tagged pc0 FETCH INST0 REFI0).
-     assert (ti0 = INSTR (Some pc0)).
-     { rewrite GET in PC0; inversion PC0; auto. }
-     subst.
-     destruct tpc1.
-    { (*case sst0 has a pc tag set*)
-      destruct o; [idtac | inversion NEXT0].
-      destruct (valid_jmp w0 pc0); [idtac | inversion NEXT0].
-      simpl in NEXT0. inversion NEXT0; subst.
-      destruct ti. (*could avoid this*)
-      - (*case ti is tagged as an instr*)
-        destruct o.
-        + (*case ti has an id - only valid case since we are coming from a jump*)
-          assert (w = pc) by (eapply id_hypothesis; eauto). subst w.
-          assert (r = r0) by (rewrite INST0 in INST1; inversion INST1; auto); subst r0.
-          assert (EQ := reg_refined_values r REFR0 RW RW0). subst apc.
-          rewrite VALID in NEXT. match_inv.
-        + simpl in NEXT; inversion NEXT.
-      - simpl in NEXT; inversion NEXT.
-    }
-    { simpl in NEXT0. inversion NEXT0; subst.
-      destruct ti. (*could avoid this*)
-      - (*case ti is tagged as an instr*)
-        destruct o.
-        + (*case ti has an id - only valid case since we are coming from a jump*)
-          assert (w = pc) by (eapply id_hypothesis; eauto). subst w.
-          assert (r = r0) by (rewrite INST0 in INST1; inversion INST1; auto); subst r0.
-          assert (EQ := reg_refined_values r REFR0 RW RW0). subst apc.
-          rewrite VALID in NEXT. simpl in NEXT. inversion NEXT. match_inv.
-        + simpl in NEXT; inversion NEXT.
-      - simpl in NEXT; inversion NEXT.
-    }
-  * 
-
-
-
-     simpl in H5. inversion H5; subst.
-     rewrite INST0 in INST1. inversion INST1; subst.
-     
-
-     
-     destruct tpc1.
-    { (*case sst0 has a pc tag set*)
-      destruct o; [idtac | inversion NEXT0].
-      destruct (valid_jmp w0 pc0); [idtac | inversion NEXT0].
-      simpl in NEXT0. inversion NEXT0; subst.
-      destruct ti. (*could avoid this*)
-      - (*case ti is tagged as an instr*)
-        destruct o.
-        + (*case ti has an id - only valid case since we are coming from a jump*)
-          assert (w = pc) by (eapply id_hypothesis; eauto). subst w.
-          assert (r = r0) by (rewrite INST0 in INST1; inversion INST1; auto); subst r0.
-          assert (EQ := reg_refined_values r REFR0 RW RW0). subst apc.
-          rewrite VALID in NEXT. match_inv.
-        + simpl in NEXT; inversion NEXT.
-      - simpl in NEXT; inversion NEXT.
-    }
-     
-  
-
-
-
-  (*nop*)
-  unfold refine_violation_state in REF.
-  destruct REF as [? [ast0 [sst0 REF]]].
-  destruct ast0 as [[[[imem0 dmem0] aregs0] apc0] b0].
-  destruct REF as [? [? [? [? ?]]]]; subst.
-  unfold Symbolic.next_state_pc in NEXT. unfold Symbolic.next_state in NEXT.
-  simpl in NEXT.
-  unfold refine_normal_state in H3. 
-  destruct sst0 as [mem0 regs0 [pc0 tpc0] ?]. 
-  destruct H3 as [? [? [? [? ?]]]].
-  inversion H1; subst.
-  * (*case amachine took a jump*)
-    inversion H2; inversion ST; subst;
-    (*uninteresting cases*)
-    match goal with 
-        | [H: refine_imemory ?Imem ?Mem, H1: Abstract.get_imem ?Imem ?Pc = Some ?I,
-           H2: Symbolic.get_mem ?Mem ?Pc = Some ?I'@_ |- _] => 
-          destruct (imem_refined_instructions Pc H H1 H2); try congruence
-    end. 
-    (*case smachine took a jump too*)
-    unfold Symbolic.next_state_pc in NEXT0.
-    unfold Symbolic.next_state in NEXT0. simpl in NEXT0.
-    assert (GET := jump_tagged pc0 FETCH INST0 H5). 
-    assert (ti0 = (INSTR (Some pc0))).
-    { rewrite GET in PC0. inversion PC0; auto. }
-    subst ti0.
-    destruct tpc1.
-    { (*case sst0 has a pc tag set*)
-      destruct o; [idtac | inversion NEXT0].
-      destruct (valid_jmp w0 pc0); [idtac | inversion NEXT0].
-      simpl in NEXT0. inversion NEXT0; subst.
-      destruct ti. (*could avoid this*)
-      - (*case ti is tagged as an instr*)
-        destruct o.
-        + (*case ti has an id - only valid case since we are coming from a jump*)
-          assert (w = pc) by (eapply id_hypothesis; eauto). subst w.
-          assert (r = r0) by (rewrite INST0 in INST1; inversion INST1; auto); subst r0.
-          assert (EQ := reg_refined_values r H7 RW RW0). subst apc.
-          rewrite VALID in NEXT. simpl in NEXT. inversion NEXT.
-        + simpl in NEXT; inversion NEXT.
-      - simpl in NEXT; inversion NEXT.
-    }
-    { simpl in NEXT0. inversion NEXT0; subst.
-      destruct ti. (*could avoid this*)
-      - (*case ti is tagged as an instr*)
-        destruct o.
-        + (*case ti has an id - only valid case since we are coming from a jump*)
-          assert (w = pc) by (eapply id_hypothesis; eauto). subst w.
-          assert (r = r0) by (rewrite INST0 in INST1; inversion INST1; auto); subst r0.
-          assert (EQ := reg_refined_values r H7 RW RW0). subst apc.
-          rewrite VALID in NEXT. simpl in NEXT. inversion NEXT.
-        + simpl in NEXT; inversion NEXT.
-      - simpl in NEXT; inversion NEXT.
-    }
-  * (*case amachine took a JAL*)
-    inversion H2; inversion ST; subst;
-    (*uninteresting cases*)
-    match goal with 
-        | [H: refine_imemory ?Imem ?Mem, H1: Abstract.get_imem ?Imem ?Pc = Some ?I,
-           H2: Symbolic.get_mem ?Mem ?Pc = Some ?I'@_ |- _] => 
-          destruct (imem_refined_instructions Pc H H1 H2); try congruence
-    end.
-   
-    
-      
-
-(* ast ~v sst,  ast = (imem,dmem,reg,apc,false) 
-   sst -> sst'
-  --------------------
-   ast ~v sst => ast0 ~ sst0, ast0 -> ast, sst0 -> sst, valid_jmp apc0 apc = false
-   
-   1. analysis on sst -> sst'
-      a. case tpc = INSTR (Some n) and ti = INTR (Some m). By hypothesis n = apc0, m = apc.
-      b. case tpc = DATA. by SSTEP, sst' rvec results in INSTR. Contadiction.
-    
-
-*)
 
 Theorem backwards_simulation ast sst sst' :
   refine_state ast sst ->
@@ -618,7 +362,239 @@ Theorem backwards_simulation ast sst sst' :
     Abstract.step atable valid_jmp ast ast' /\
     refine_state ast' sst'.
 Proof.
-Admitted.
- 
+  intros REF SSTEP.
+  destruct ast as [[[[imem dmem] aregs] apc] b].
+  destruct b.
+  (* Focus 2. *)
+  (* inversion SSTEP; subst; *)
+  (* destruct REF as [REFI [REFD [REFR [REFPC CORRECTNESS]]]]; *)
+  (* destruct (CORRECTNESS i ti PC) as [? ABSURD]; *)
+  (* (*unfoldings and case analysis on tags*) *)
+  (* repeat ( *)
+  (*     match goal with *)
+  (*       | [H: refine_pc _ _ |- _] => unfold refine_pc in H; simpl in H *)
+  (*       | [H: Symbolic.next_state_pc _ _ _ = _ |- _] => *)
+  (*         unfold Symbolic.next_state_pc in H *)
+  (*       | [H: Symbolic.next_state_reg _ _ _ _ = _ |- _] => *)
+  (*         unfold Symbolic.next_state_reg in H *)
+  (*       | [H: Symbolic.next_state_reg_and_pc _ _ _ _ _ = _ |- _] => *)
+  (*         unfold Symbolic.next_state_reg_and_pc in H *)
+  (*       | [H: Symbolic.next_state _ _ _ = Some _ |- _] => *)
+  (*         unfold Symbolic.next_state in H; simpl in H; match_inv *)
+  (*     end); subst; assert (false = true); *)
+  (* try match goal with *)
+  (*     | [H: _ -> false = true |- false = true] => apply H *)
+  (* end; *)
+  (* repeat match goal with *)
+  (*     | [|- forall _, _] => intros *)
+  (*     | [H: INSTR _ = INSTR _ |- _] => inversion H; subst; clear H *)
+  (*     | [H: DATA = INSTR _ |- _] => inversion H *)
+  (*     | [|- exists _, _] => eexists; eauto *)
+  (* end; try discriminate. *)
+  (*syscalls stuck*)
+(*1st case*)
+  - inversion SSTEP; subst;
+    destruct REF as [REFI [REFD [REFR [REFPC CORRECTNESS]]]];
+  (*unfoldings and case analysis on tags*)
+  repeat (
+      match goal with
+        | [H: refine_pc _ _ |- _] => unfold refine_pc in H; simpl in H
+        | [H: Symbolic.next_state_pc _ _ _ = _ |- _] => 
+          unfold Symbolic.next_state_pc in H
+        | [H: Symbolic.next_state_reg _ _ _ _ = _ |- _] => 
+          unfold Symbolic.next_state_reg in H
+        | [H: Symbolic.next_state_reg_and_pc _ _ _ _ _ = _ |- _] => 
+          unfold Symbolic.next_state_reg_and_pc in H
+        | [H: Symbolic.next_state _ _ _ = Some _ |- _] =>
+          unfold Symbolic.next_state in H; simpl in H; match_inv
+      end); subst;
+  (* switch memory updates to abstract*)
+  repeat (
+      match goal with
+        | [H: upd ?Mem ?Addr ?V@_ = Some _, 
+           H1 : refine_dmemory _ ?Mem, 
+           H2: get ?Mem ?Addr = Some _ |- _] => 
+          simpl in H; 
+          destruct (refine_memory_upd Addr V H1 H2 H) as [dmem' [? ?]]
+  end);
+  (*switch memory and register reads to abstract*)
+  try match goal with
+    | [H1: refine_imemory _ ?Mem, 
+       H2: get ?Mem ?Pc = Some ?I@(INSTR _) |- _] =>
+      assert (exists id, get Mem Pc = Some I@(INSTR id)) 
+        by (eexists;eauto)
+  end;
+  (*make register gets in the form of existentials*)
+  try match goal with
+    | [H1: refine_registers _ ?Reg, H2: get ?Reg ?R = Some ?V@_,
+       H3: get ?Reg ?R' = Some ?V'@_, 
+       H4: get ?Reg ?R'' = Some ?V''@_ |- _] =>
+      assert (exists ut, get Reg R = Some V@ut) 
+        by (eexists;eauto);
+      assert (exists ut, get Reg R' = Some V'@ut) 
+        by (eexists;eauto);
+      assert (exists ut, get Reg R' = Some V'@ut) 
+        by (eexists;eauto)
+    | [H1: refine_registers _ ?Reg, H2: get ?Reg ?R = Some ?V@_,
+       H3: get ?Reg ?R' = Some ?V'@_|- _] =>
+      assert (exists ut, get Reg R = Some V@ut) 
+        by (eexists;eauto);
+      assert (exists ut, get Reg R' = Some V'@ut) 
+        by (eexists;eauto)
+    | [H1: refine_registers _ ?Reg, 
+       H2: get ?Reg ?R = Some ?V@_ |- _] =>
+      assert (exists ut, get Reg R = Some V@ut) 
+        by (eexists;eauto)
+  end;
+  (*do actual refinements*)
+  repeat match goal with
+    | [H1: refine_imemory _ ?Mem, 
+           H2: exists _, get ?Mem _ = Some _@(INSTR _) |- _] =>
+      apply H1 in H2
+    | [H1: refine_dmemory _ ?Mem, H2: get ?Mem _ = Some _@DATA |- _] => 
+      apply H1 in H2
+    | [H1: refine_registers _ ?Reg, 
+           H2: exists _, get ?Reg _ = Some _ |- _] => 
+      apply H1 in H2
+  end; 
+  (*Refine registers update - unsure about this part - it seems to still work*)
+  repeat match goal with
+    | [H: refine_registers ?Aregs ?Regs, 
+          H1: get ?Aregs ?R = Some ?Old |- _] => 
+      unfold refine_registers in H; destruct (H R Old) as [RSA RAS]; 
+      destruct RAS as [x RAS'];
+      apply RAS' in H1; fold (refine_registers Aregs Regs) in H
+    | [H: refine_registers _ _, H1: get ?Reg ?R = Some _,
+          H2: upd _ ?R ?V'@?T' = Some _ |- _] =>
+      destruct (refine_registers_upd R V' T' H H1 H2) as [aregs' [? ?]]
     
-    
+         end; auto;   
+  destruct (refine_syscalls_correct) as [DOMAIN SYSCALLREF];
+  (* put into context stuff required for syscalls *)
+    try
+      match goal with
+        | [H: decode_instr _ = Some (Jal _ _ ),
+           H1: Symbolic.get_syscall _ ?W = Some _
+           |- _] =>
+          assert (EGETCALL: exists sc, Symbolic.get_syscall stable W = Some sc)
+            by (eexists; eauto);
+            destruct (DOMAIN W) as [ASDOM SADOM];
+            apply SADOM in EGETCALL; destruct EGETCALL;
+            assert (REF: refine_state (imem,dmem,aregs,pc,true) (Symbolic.State mem reg pc@tpc int))
+                     by (repeat (split; auto));
+            destruct (syscalls_backwards_simulation (imem,dmem,aregs,pc,true) 
+                                                    (Symbolic.State mem reg pc@tpc int)
+                                                    W
+                                                    refine_syscalls_correct H1
+                                                    REF CALL) as
+                [ac [ast' [GETCALL' [CALL' FINALREF]]]];
+            destruct ast' as [[[[imem' dmem'] aregs'] apc'] b];
+            destruct (syscall_sem ac (imem,dmem,aregs,pc,true) CALL') as 
+                [? [? ?]];
+            subst
+      end;
+  (*handle abstract steps*)
+  repeat (match goal with 
+    | [|- exists _,  _ /\ _] => eexists; split
+    | [|- Abstract.step _ _ _ _] => econstructor(eassumption)
+    | [H: decode_instr _ = Some (Load _ _ _) |- Abstract.step _ _ _ _] => 
+      eapply Abstract.step_load; eauto
+    | [H: get ?Mem ?Addr = Some ?V@?TG, H1: refine_imemory _ _, 
+       H2: refine_dmemory _ _ 
+       |- get _ ?Addr =  _ \/ get _ ?Addr = _] => (*for load*)
+      destruct TG; 
+        [left; 
+          assert(MEMLOAD: exists id, get Mem Addr = Some V@(INSTR id)) 
+           by (eexists; eauto); apply H1 in MEMLOAD; eassumption | 
+         right; apply H2 in H; eassumption]
+    | [H: decode_instr _ = Some (Store _ _ _) |- Abstract.step _ _ _ _] => 
+      eapply Abstract.step_store; eauto
+    | [H: decode_instr _ = Some (Jump _ _ ) |- Abstract.step _ _ _ _] => 
+      eapply Abstract.step_jump; eauto
+    | [H: decode_instr _ = Some (Bnz _ _ _) |- Abstract.step _ _ _ _] =>
+      eapply Abstract.step_bnz; eauto
+    | [H: decode_instr _ = Some (Jal _ _ ), H1: Symbolic.get_syscall _ _ = None 
+       |- Abstract.step _ _ _ _] =>
+      eapply Abstract.step_jal; eauto
+    | [H: decode_instr _ = Some (Jal _ _ ), H1: Symbolic.get_syscall _ _ = Some _
+       |- Abstract.step _ _ _ _] =>
+      eapply Abstract.step_syscall; eauto
+         end);
+  unfold refine_state;
+  (*handle final state refinement*)
+  repeat (match goal with
+    | [H: decode_instr _ = Some (Jump _ _) |- refine_state (_,_,_,_, valid_jmp ?Pc ?W) _] =>
+      remember (valid_jmp Pc W) as b; destruct b; [left; unfold refine_normal_state; repeat (split; auto) | idtac]
+    | [H: false = valid_jmp ?Pc ?W |- refine_state (_,_,_,_, false) _] =>
+      idtac
+    | [|- _ /\ _] => split; [eauto | idtac]
+    | [H: decode_instr _ = Some (Jump _ _) |- Abstract.step _ _ _ (_,_,_,_,false)] =>
+      eapply Abstract.step_jump; eauto
+    | [H: refine_imemory ?Imem ?Mem |- refine_imemory ?Imem ?Mem] => assumption
+    | [H: refine_imemory ?Imem ?Mem |- refine_imemory ?Imem ?Mem'] => 
+        eapply imem_upd_preservation; eauto
+    | [|- refine_pc _ _] => unfold refine_pc; simpl; auto
+   end); 
+  (*handle the correctness part*)
+  repeat match goal with
+    | [|- forall _, _] => intros
+    | [|- _ <-> _] => simpl; split; try discriminate
+    | [|- true = true] => reflexivity
+  end;
+  repeat match goal with
+           | [H: refine_dmemory dmem ?Mem |- get ?Mem _ = Some _] => 
+             eapply H; eauto
+         end; auto;
+  (*jump/jal related stuff*)
+    (*no syscall*)
+    try 
+      match goal with
+        | [H: Symbolic.get_syscall _ ?W = None 
+           |- Abstract.get_syscall _ ?W = None] =>
+          eapply same_domain_total in DOMAIN; eapply DOMAIN; assumption
+      end;
+    repeat (
+        match goal with
+          | [H: INSTR ?V = INSTR ?V |- _] => idtac
+          | [H: INSTR _ = INSTR _ |- _] => inversion H; subst
+        end);
+    try match goal with
+          | [H: get ?Mem ?Pc = Some ?I@(INSTR (Some _)), 
+             H1: decode_instr ?I = Some (Jump _ ?R), 
+             H2: get ?Reg ?R = Some ?W@_,
+             H3: get ?Mem ?W = Some _ 
+             |- _] =>
+               assert (EQ := jump_target_tagged Pc Mem Reg H H1 H2 H3);
+               assert (EQ' := jump_tagged Pc Mem H H1); inversion EQ'; subst
+          | [H: get ?Mem ?Pc = Some ?I@(INSTR (Some _)), 
+             H1: decode_instr ?I = Some (Jal _ ?R), 
+             H2: get ?Reg ?R = Some ?W@_,
+             H3: get ?Mem ?W = Some _,
+             H4: Symbolic.get_syscall stable ?W = None
+             |- _] =>
+               assert (EQ := jal_target_tagged Pc Mem Reg H H1 H2 H3 H4);
+               assert (EQ' := jal_tagged Pc Mem H H1); inversion EQ'; subst
+        end;
+   try 
+     match goal with
+       | [|- exists _, INSTR (Some ?W) = INSTR _ /\ valid_jmp _ _ = true] =>
+         exists W; split; auto
+       | [H: forall _, INSTR (Some ?W) = INSTR (Some _) -> _ 
+                              |- valid_jmp _ _ = true] =>
+         assert (TRUE: INSTR (Some W) = INSTR (Some W)) by reflexivity;
+         destruct (H W TRUE) as [dst [TI VALID]]; inversion TI; auto
+     end. 
+    (*more system calls*)
+    { destruct ti.
+    + assert (EQ := jal_tagged pc mem PC INST).
+      apply REFI; eexists; eauto.
+    + simpl in ALLOWED; match_inv.
+    } 
+    destruct sst' as [mem' reg' [pc' tpc'] int'].
+    destruct FINALREF as [REFI' [REFD' [REFR' [REFPC' CORRECTNESS']]]].
+    repeat(split; auto).
+    (*syscall correctness*)
+     (*not sure if provable right now*)
+Admitted.   
+
+End Refinement.
